Add mutual recursion version of collect with program fixpoint

src/Query.v
@@ -22,280 +22,42 @@ Section Query.
 
 
   Variables Name Vals : ordType.
-  
-  Inductive Query : Type :=
-  | SingleField : Name -> {fmap Name -> Vals} -> Query
-  | LabeledField : Name -> Name -> {fmap Name -> Vals} -> Query
-  | NestedField : Name -> {fmap Name -> Vals} -> Query -> Query
-  | NestedLabeledField : Name -> Name -> {fmap Name -> Vals} -> Query -> Query
-  | InlineFragment : Name -> Query -> Query    (* Check it's named type and not list *)
-  | SelectionSet : list Query -> Query.   (* seq Query but not empty... *)
+
+  Inductive SelectionSet : Type :=
+  | SingleSelection : Query -> SelectionSet
+  | MultipleSelection : Query -> SelectionSet -> SelectionSet
+  with Query : Type :=
+       | SingleField : Name -> {fmap Name -> Vals} -> Query
+       | LabeledField : Name -> Name -> {fmap Name -> Vals} -> Query
+       | NestedField : Name -> {fmap Name -> Vals} -> SelectionSet -> Query
+       | NestedLabeledField : Name -> Name -> {fmap Name -> Vals} -> SelectionSet -> Query
+       | InlineFragment : Name -> SelectionSet -> Query.
 
 
   Unset Elimination Schemes.
   Inductive ResponseObject : Type :=
-  | Empty : ResponseObject
-  | Null : Name -> ResponseObject
-  | SingleResult : Name -> Vals -> ResponseObject
-  | ListResult : Name -> list Vals -> ResponseObject
-  | NestedResult : Name -> ResponseObject -> ResponseObject
-  | NestedListResult : Name -> list ResponseObject -> ResponseObject
-  | ResponseList : list ResponseObject -> ResponseObject.
+  | SingleResponse : Result -> ResponseObject
+  | MultipleResponses : Result -> ResponseObject -> ResponseObject
+  with Result : Type :=
+  | Empty : Result
+  | Null : Name -> Result
+  | SingleResult : Name -> Vals -> Result
+  | ListResult : Name -> list Vals -> Result
+  | NestedResult : Name -> ResponseObject -> Result
+  | NestedListResult : Name -> list ResponseObject -> Result.
   Set Elimination Schemes.
 
-  
-  Definition ResponseObject_rect P Pl IH_Empty IH_Null IH_SingleResult IH_ListResult IH_NestedResult IH_NestedListResult IH_ResponseList IH_Nil IH_Cons :=
-    fix loop (r : ResponseObject) : P r :=
-      match r with
-      | Empty => IH_Empty
-      | Null l => IH_Null l
-      | SingleResult l v => IH_SingleResult l v
-      | ListResult l vals => IH_ListResult l vals
-      | NestedResult l r' => IH_NestedResult l r' (loop r')
-      | NestedListResult l rs => IH_NestedListResult l rs
-                                                    ((fix F s : Pl s :=
-                                                        match s with
-                                                        | [::] => IH_Nil
-                                                        | hd :: tl => IH_Cons hd (loop hd) tl (F tl)
-                                                        end) rs)
-        
-      | ResponseList rs => IH_ResponseList rs ((fix F s : Pl s :=
-                                                        match s with
-                                                        | [::] => IH_Nil
-                                                        | hd :: tl => IH_Cons hd (loop hd) tl (F tl)
-                                                        end) rs)
-      end.
-
-  Definition ResponseObject_rec (P : ResponseObject -> Set) := @ResponseObject_rect P.
-
-  Definition ResponseObject_ind P (Pl : seq.seq ResponseObject -> Prop) IH_Empty IH_Null IH_SingleResult IH_ListResult IH_NestedResult IH_NestedListResult IH_ResponseList IH_Nil IH_Cons :=
-    fix loop (r : ResponseObject) : P r : Prop :=
-      match r with
-      | Empty => IH_Empty
-      | Null l => IH_Null l
-      | SingleResult l v => IH_SingleResult l v
-      | ListResult l vals => IH_ListResult l vals
-      | NestedResult l r' => IH_NestedResult l r' (loop r')
-      | NestedListResult l rs => IH_NestedListResult l rs
-                                                    ((fix F s : Pl s :=
-                                                        match s with
-                                                        | [::] => IH_Nil
-                                                        | hd :: tl => IH_Cons hd (loop hd) tl (F tl)
-                                                        end) rs)
-      | ResponseList rs => IH_ResponseList rs ((fix F s : Pl s :=
-                                                        match s with
-                                                        | [::] => IH_Nil
-                                                        | hd :: tl => IH_Cons hd (loop hd) tl (F tl)
-                                                        end) rs)
-      end.
+         
 
   
   
-  (* Right now it is returning a GenTree.tree (Name * Name * {fmap Name -> Vals})
-     
-     The tuple represents (label, field name, args) but for the case of unlabeled fields
-     there is some redundancy, where the label is the same as the field name.
-
-     Another option would be to return a GenTree.tree ((Name, {fmap ...}) + (Name, Name, {fmap ...}))
-     but this option doesn't allow (currently) to define Query as ordType, due to sum type
-     not being of ordType itself.
-   
-    Fixpoint tree_of_query query : GenTree.tree (Name * Name * {fmap Name -> Vals})  :=
-    match query with
-    | SingleField name args => GenTree.Node 0 [:: GenTree.Leaf (name, name, args)]
-    | LabeledField label name args => GenTree.Node 1 [:: GenTree.Leaf (label, name, args)]
-    | NestedField name args ϕ => GenTree.Node 2 [:: GenTree.Leaf (name, name, args);
-                                                  tree_of_query ϕ]
-    | NestedLabeledField label name args ϕ =>  GenTree.Node 3 [:: GenTree.Leaf (label, name, args);
-                                                                tree_of_query ϕ]
-    | InlineFragment t ϕ => GenTree.Node 4 [:: GenTree.Leaf (t, t, emptym) ;
-                                             tree_of_query ϕ]
-    | SelectionSet ϕ ϕ' => GenTree.Node 5 [:: tree_of_query ϕ ; tree_of_query ϕ']
-    end.
-
-  Fixpoint query_of_tree (tree : GenTree.tree (Name * Name * {fmap Name -> Vals})) : option Query :=
-    match tree with
-    | GenTree.Node 0 [:: GenTree.Leaf (_, name, args)] => Some (SingleField name args)
-    | GenTree.Node 1 [:: GenTree.Leaf (label, name, args)] => Some (LabeledField label name args)
-    | GenTree.Node 2 [:: GenTree.Leaf (_, name, args); t'] =>
-      if (query_of_tree t') is Some q then
-        Some (NestedField name args q)
-      else
-        None
-    | GenTree.Node 3 [:: GenTree.Leaf (label, name, args); t'] =>
-      if (query_of_tree t') is Some q then
-        Some (NestedLabeledField label name args q)
-      else
-        None
-    |  GenTree.Node 4 [:: GenTree.Leaf (_, ty, emptym); t'] =>
-       if (query_of_tree t') is Some q then
-         Some (InlineFragment (NamedType ty) q)
-       else
-         None
-    | GenTree.Node 5 [:: t' ; t''] =>
-      match (query_of_tree t'), (query_of_tree t'') with
-      | Some q, Some q' => Some (SelectionSet q q')
-      | _, _ => None
-      end
-    | _ => None
-    end.
-
-  Lemma pcan_tree_of_query : pcancel tree_of_query query_of_tree.
-  Proof.
-    elim=> //.
-      by move=> s args q /= ->.
-      by move=> l s args q /= ->.
-      by move=> t q /= ->.
-      by move=> q H q' H' /=; rewrite H H'.
-  Qed.
-
-   Definition query_eqMixin := PcanEqMixin pcan_tree_of_query.
-   Canonical query_eqType := EqType Query query_eqMixin.
-   Definition query_choiceMixin := PcanChoiceMixin pcan_tree_of_query.
-   Canonical query_choiceType := ChoiceType Query query_choiceMixin.
-   Definition query_ordMixin := PcanOrdMixin pcan_tree_of_query.
-   Canonical query_ordType := OrdType Query query_ordMixin.
-
-*)
-
-   
-   
-   Fixpoint tree_of_response response : GenTree.tree (Name + (Vals + seq.seq Vals)) :=
-     match response with
-     | Empty => GenTree.Node 0 [::]
-     | Null l => GenTree.Node 1 [:: GenTree.Leaf (inl l)]
-     | SingleResult l val => GenTree.Node 2 [:: GenTree.Leaf (inl l) ; GenTree.Leaf (inr (inl val))]
-     | ListResult l vals => GenTree.Node 3 [:: GenTree.Leaf (inl l) ; GenTree.Leaf (inr (inr vals))]
-     | NestedResult l q => GenTree.Node 4 [:: GenTree.Leaf (inl l) ; tree_of_response q]
-     | NestedListResult l qs => GenTree.Node 5 (GenTree.Leaf (inl l) :: (map tree_of_response qs))
-     | ResponseList rs => GenTree.Node 6 (map tree_of_response rs)
-     end.
-
-
-   Fixpoint response_of_tree (t : GenTree.tree (Name + (Vals + seq.seq Vals))) :=
-     match t with
-     | GenTree.Node 0 [::] => Empty
-     | GenTree.Node 1 [:: GenTree.Leaf (inl l)] => Null l
-     | GenTree.Node 2 [:: GenTree.Leaf (inl l) ; GenTree.Leaf (inr (inl val))] => SingleResult l val
-     | GenTree.Node 3 [:: GenTree.Leaf (inl l) ; GenTree.Leaf (inr (inr vals))] => ListResult l vals
-     | GenTree.Node 4 [:: GenTree.Leaf (inl l) ; t'] => NestedResult l (response_of_tree t')
-     | GenTree.Node 5 (GenTree.Leaf (inl l) :: t') => NestedListResult l (map response_of_tree t')
-     | GenTree.Node 6 t' => ResponseList (map response_of_tree t')
-     | _ => Empty
-     end.
-
-   Lemma tree_of_responseK : cancel tree_of_response response_of_tree.
-   Proof.
-     rewrite /cancel.
-     eapply ResponseObject_ind => //.
-     Admitted. (*
-     apply (ResponseObject_ind  (fun (rs : list ResponseObject) =>  (map response_of_tree (map tree_of_response rs)) = rs)).
-     apply: (ResponseObject_ind (fun (rs : list ResponseObject) => map response_of_tree (map tree_of_response rs) = rs)).
-     
-       by move=> s r /= ->.
-       move=> s rs IH /=. elim: rs IH => [|r rs' IH] //=.
-       by move=> [-> /IH {IH} IH]; case: IH => ->.
-       by move=> r IH r' IH' /=; rewrite IH IH'.
-   Qed.*)
-
-   Definition response_eqMixin := CanEqMixin tree_of_responseK.
-   Canonical response_eqType := EqType ResponseObject response_eqMixin.
-   Definition response_choiceMixin := CanChoiceMixin tree_of_responseK.
-   Canonical response_choiceType := ChoiceType ResponseObject response_choiceMixin.
-   Definition response_ordMixin := CanOrdMixin tree_of_responseK.
-   Canonical response_ordType := OrdType ResponseObject response_ordMixin.
-
-
-   (*
-  Fixpoint isFieldSelection query :=
-    match query with
-    | SingleField _ _ => true
-    | LabeledField _ _ _ => true
-    | NestedField _ _ _ => true
-    | NestedLabeledField _ _ _ _ => true
-    | SelectionSet hd tl => isFieldSelection hd && isFieldSelection tl
-    | _ => false
-    end.
-
-  Fixpoint isInlineFragmentSelection query :=
-    match query with
-    | InlineFragment _ _ => true
-    | SelectionSet hd tl => isInlineFragmentSelection hd && isInlineFragmentSelection tl
-    | _ => false
-    end.
-  
-  Inductive GroundTypedNormalForm : Query -> Prop :=
-  | GT_Field : forall f args,
-      GroundTypedNormalForm (SingleField f args)
-
-  | GT_LabeledField : forall label f args,
-      GroundTypedNormalForm (LabeledField label f args)
-
-  | GT_NestedField : forall f args ϕ,
-      GroundTypedNormalForm ϕ ->
-      GroundTypedNormalForm (NestedField f args ϕ)
-
-  | GT_NestedLabeledField : forall label f args ϕ,
-      GroundTypedNormalForm ϕ ->
-      GroundTypedNormalForm (NestedLabeledField label f args ϕ)
-
-  | GT_InlineFragment : forall t ϕ,
-      (* isObjectType schema t *)
-      isFieldSelection ϕ ->
-      GroundTypedNormalForm ϕ ->
-      GroundTypedNormalForm (InlineFragment t ϕ)
-
-  | GT_SelectionSet : forall ϕ ϕ',
-      (isFieldSelection ϕ && isFieldSelection ϕ') || (isInlineFragmentSelection ϕ && isInlineFragmentSelection ϕ') ->
-      GroundTypedNormalForm ϕ ->
-      GroundTypedNormalForm ϕ' ->
-      GroundTypedNormalForm (SelectionSet ϕ ϕ').
-
-  Fixpoint is_ground_typed_normal_form query :=
-    match query with
-    | NestedField _ _ ϕ => is_ground_typed_normal_form ϕ
-    | NestedLabeledField _ _ _ ϕ => is_ground_typed_normal_form ϕ
-    | InlineFragment _ ϕ => isFieldSelection ϕ && is_ground_typed_normal_form ϕ
-    | SelectionSet ϕ ϕ' => ((isFieldSelection ϕ && isFieldSelection ϕ')
-                           || (isInlineFragmentSelection ϕ && isInlineFragmentSelection ϕ'))
-                            && is_ground_typed_normal_form ϕ && is_ground_typed_normal_form ϕ'
-    | _ => true
-    end.
-
-
-
-
-    Lemma and_foldr_forall (T : eqType) (P : T -> Prop) (s : seq.seq T) :
-      foldr (fun t => and (P t)) True s -> forall t, In t s -> P t.
-    Proof.
-    elim: s => [| x s' IH] //=.
-    move=> [Hpx Hf] t.
-    by move=> [<-| Hs]; [ | apply (IH Hf t Hs)].
-    Qed.
-    *)
-
-   Implicit Type query : Query.
-
-   Definition is_selection_set query :=
-     if query is SelectionSet _ then true else false.
-   
-   Fixpoint is_query_wf query :=
-     match query with
-     | NestedField _ _ q => is_query_wf q
-     | NestedLabeledField _ _ _ q => is_query_wf q
-     | InlineFragment _ q => is_query_wf q
-     | SelectionSet q => all (fun q' => ~~(is_selection_set q') && is_query_wf q') q
-     | _ => true
-     end.
-
-   Structure wfQuery := WFQuery {
-                           query : Query;
-                           _ : is_query_wf query
-                         }.
 
   
 End Query.
 
+
+Arguments SingleSelection [Name Vals].
+Arguments MultipleSelection [Name Vals].
 Arguments Query [Name Vals].
 Arguments SingleField [Name Vals].
 Arguments LabeledField [Name Vals].
@@ -308,103 +70,6 @@ Arguments SelectionSet [Name Vals].
 Arguments ResponseObject [Name Vals].
 Arguments Null [Name Vals].
 Arguments Empty [Name Vals].
+Arguments SingleResult [Name Vals].
 
 
-
-
-  (*
-  Fixpoint query_eq q1 q2 :=
-    match q1, q2 with
-    | SingleField name args, SingleField name' args' => (name == name') && (args == args')
-    | LabeledField label name args, LabeledField label' name' args' => (label == label') && (name == name') && (args == args')
-    | NestedField name args ϕ, NestedField name' args' ϕ' => (name == name') && (args == args') && query_eq ϕ ϕ'
-    | NestedLabeledField label name args ϕ, NestedLabeledField label' name' args' ϕ' =>
-      (label == label') && (name == name') && (args == args') && query_eq ϕ ϕ'
-    | InlineFragment t ϕ, InlineFragment t' ϕ' => (t == t') && query_eq ϕ ϕ'
-    | SelectionSet ϕ ϕ', SelectionSet ψ ψ' => (query_eq ϕ ψ) &&  (query_eq ϕ' ψ')
-    | _,  _ => false
-    end.
-
-
-  Lemma query_eqP : Equality.axiom query_eq.
-  Proof.
-    rewrite /Equality.axiom.
-    move=> x y; apply: (iffP idP) => [| <- {y}].
-    move: y; elim: x.
-    by move=> n args; case=> n' args' //=; move/andP=> [/eqP -> /eqP ->].
-    by move=> l n args; case=> l' n' args' //=; move/andP=> [/andP [/eqP -> /eqP ->] /eqP ->].
-    move=> n args q IH; case=> // => n' args' q' /=; move/andP=> [/andP [/eqP -> /eqP ->] H].
-      by apply IH in H; rewrite H.
-    move=> l n args q IH; case=> // => l' n' args' q' /=; move/andP=> [/andP [/andP [/eqP -> /eqP ->] /eqP ->] H].
-      by apply IH in H; rewrite H.
-    move=> t q IH; case=> // => t' q' /=; move/andP=> [/eqP -> H].
-      by apply IH in H; rewrite H.
-    move=> q IH q' IH'. case=> // => q'' q''' //=. move/andP=> [H1 H2].
-    by apply IH in H1; apply IH' in H2; rewrite H1 H2. 
-    elim: x => /=.
-    by move=> s f; rewrite !eqxx.
-    by move=> l s f; rewrite !eqxx.
-    by move=> s f q IH; rewrite !eqxx.
-    by move=> l s f q IH; rewrite !eqxx.
-    by move=> t q IH; rewrite !eqxx.
-    move=> q IH q' IH'. rewrite !eqxx. *)
-
-
-
-(*
-
-   Fixpoint response_eq r1 r2 :=
-     match r1, r2 with
-     | Empty, Empty => true
-     | Null l, Null l' => l == l'
-     | SingleResult l val, SingleResult l' val' => (l == l') && (val == val')
-     | ListResult l vals, ListResult l' vals' => (l == l') && (vals == vals')
-     | NestedResult l r1', NestedResult l' r2' => (l == l') && (response_eq r1' r2')
-     | NestedListResult l rs, NestedListResult l' rs' =>
-       let fix loop s1 s2 :=
-           match s1, s2 with
-           | [::], [::] => true
-           | r1 :: s1, r2 :: s2 => if response_eq r1 r2 then loop s1 s2 else false
-           | _, _ => false
-           end
-       in
-       (l == l') && loop rs rs'
-     | ResponseList r1' r1'', ResponseList r2' r2'' => (response_eq r1' r2') && (response_eq r1'' r2'')
-     | _, _ => false
-     end.
-
-   Lemma response_eqP : Equality.axiom response_eq.
-   Proof.
-     rewrite /Equality.axiom => x y.
-     apply: (iffP idP) => [|<-].
-     move: y;  elim: x.   
-       by case.
-       by move=> l; case=> //; move=> l' /=; move/eqP=> ->.
-       by move=> l v; case=> // l' v' /=; by move/andP=> [/eqP -> /eqP ->].
-       by move=> l vals; case=> // l' vals' /=; move/andP=> [/eqP -> /eqP ->].
-       move=> l r IH; case=> // l' r' /=; move/andP=> [/eqP -> H].
-         by apply IH in H; rewrite H.
-       move=> l rs IH. case=> // l' rs' /=.
-         move/andP=> [/eqP ->].
-         elim: rs rs' IH => [| r0 rs0 IH] [| r1 rs1] //=.
-         move=> [H /IH {IH} IH] /=.
-         case E : (response_eq r0 r1) => //= /IH.
-         apply H in E; rewrite E.
-         by case=> ->.
-       move=> r IH r' IH'; case=> // => r2 r2' /=; move/andP=> [H1 H2].
-         by apply IH in H1; apply IH' in H2; rewrite H1 H2.
-     elim: x => //=.
-       by move=> l v; rewrite !eqxx.    
-       by move=> l vals; rewrite !eqxx.
-       by move=> l r; rewrite !eqxx.
-       move=> l vals IH /=; elim: vals IH => [| r rs IH] //=.
-         by rewrite !eqxx.
-         by move=> [H]; rewrite H.
-       by move=> r IH r' IH'; rewrite IH IH'.
-   Qed.
-
-   
-   Definition response_eqMixin := Equality.Mixin response_eqP.
-   Canonical response_eqType := EqType ResponseObject response_eqMixin.
-   
- *)
