src/QueryAux.v
@@ -14,43 +14,69 @@ Section QueryAux.
 
   Variables Name Vals : ordType.
 
+  Implicit Type selection : @SelectionSet Name Vals.
   Implicit Type query : @Query Name Vals.
   Implicit Type response : @ResponseObject Name Vals.
+  Implicit Type result : @Result Name Vals.
   
-  Fixpoint query_size query : nat :=
-    match query with
-    | NestedField _ _ q' => 1 + (query_size q')
-    | NestedLabeledField _ _ _ q' => 1 + (query_size q')
-    | InlineFragment _ q' => 1 + (query_size q')
-    | SelectionSet q => sumn (map query_size q)
-    | _ => 1
-    end.
+  Fixpoint selection_size selection : nat :=
+    match selection with
+    | SingleSelection q => query_size q
+    | MultipleSelection q tl => query_size q + selection_size tl
+    end
+  with query_size query : nat :=
+         match query with
+         | NestedField _ _ q' => 1 + (selection_size q')
+         | NestedLabeledField _ _ _ q' => 1 + (selection_size q')
+         | InlineFragment _ q' => 1 + (selection_size q')
+         | _ => 1
+         end.
  
-  
-  Fixpoint app_response (r1 r2 : @ResponseObject Name Vals) : ResponseObject :=
-    match r1, r2 with
-    | ResponseList rs, ResponseList rs' => ResponseList (rs ++ rs')
-    | ResponseList rs, _ => ResponseList (rs ++ [:: r2])
-    | _, ResponseList rs' => ResponseList (r1 :: rs')
-    | _, _ => ResponseList [:: r1; r2]
-    end.
+ 
 
   Fixpoint response_size response : nat :=
     match response with
+    | SingleResponse r => result_size r
+    | MultipleResponses hd tl => result_size hd + response_size tl
+    end
+  with result_size result : nat :=
+    match result with
     | Empty => 1
     | Null _ => 3
     | SingleResult _ _ => 3
     | ListResult _ vals => 4 + size vals
     | NestedResult _ r' => 4 + response_size r'
     | NestedListResult _ rs => 4 + 2 * (size rs) + sumn (map response_size rs)
-    | ResponseList rs => 1 + sumn (map response_size rs)
     end.
 
   Definition responses_size (responses : seq (@ResponseObject Name Vals)) : nat :=
     sumn (map response_size responses).
 
-
-
+  
+  Fixpoint app_responses r1 r2 : @ResponseObject Name Vals :=
+    match r1 with
+    | SingleResponse r => MultipleResponses r r2
+    | MultipleResponses hd tl => MultipleResponses hd (app_responses tl r2)
+    end.
+  (*
+  Fixpoint cleanup_empty_results response : option ResponseObject :=
+    match response with
+    | SingleResponse Empty => None
+    | SingleResponse _ => Some response
+    | MultipleResponses Empty tl => cleanup_empty_results tl
+    | MultipleResponses hd tl => Multiple                                     
+    end
+  with cleanup_empty result :=
+         match result with
+         | Empty => None
+         | NestedResult l r => let clean := (cleanup_empty_results r) in
+                              if clean is Some r' then
+                                Some (NestedResult l r')
+                              else
+                                None
+         | NestedListResult 
+         | _ => Some result *)
+  
 End QueryAux.
 
 Arguments response_size [Name Vals].
