src/Example.v
@@ -192,45 +192,42 @@ Section Example.
 
 
     
-  Let q := (NestedField "hero" [fmap ("episode", "EMPIRE")]
-                       (SelectionSet
-                          [::
-                             (SingleField "name" emptym);
-                             (NestedField "friends" emptym
-                                          (SelectionSet
-                                             [::
-                                                (InlineFragment "Human"
-                                                                (SelectionSet
-                                                                   [::
-                                                                      (LabeledField "humanFriend" "name" emptym);
-                                                                      (NestedField "starships" emptym
-                                                                                   (SelectionSet
-                                                                                      [::
-                                                                                         (LabeledField "starship" "name" emptym);
-                                                                                         (SingleField "length" emptym)
-                                                                                      ]
-                                                                                   )
-                                                                      )
-                                                                   ]
-                                                                )
-                                                );
-                                             
-                                                
-                                                (InlineFragment "Droid"
-                                                                (SelectionSet
-                                                                   [::
-                                                                      (LabeledField "droidFriend" "name" emptym);
-                                                                      (SingleField "primaryFunction" emptym)
-                                                                   ]
-                                                                )
-                                                )
-                                             ]
+    Let q := (SingleSelection
+               (NestedField "hero" [fmap ("episode", "EMPIRE")]
+                  (MultipleSelection
+                     (SingleField "name" emptym)
+                     (SingleSelection
+                        (NestedField "friends" emptym
+                           (MultipleSelection
+                              (InlineFragment "Droid"
+                                    (MultipleSelection
+                                       (LabeledField "droidFriend" "name" emptym)
+                                       (SingleSelection (SingleField "primaryFunction" emptym))
+                                    )
+                                 )
+                              (SingleSelection
+                                 (InlineFragment "Human"
+                                 (MultipleSelection
+                                    (LabeledField "humanFriend" "name" emptym)
+                                    (SingleSelection
+                                       (NestedField "starships" emptym
+                                          (MultipleSelection
+                                             (LabeledField "starship" "name" emptym)
+                                             (SingleSelection (SingleField "length" emptym))
                                           )
-                             )
-                          ]
-                       )
-          ).
-
+                                       )
+                                    )
+                                    
+                                 )
+                              )
+                              )
+                           )
+                        )
+                     )
+                  )
+               )
+            ).
+             
   (*
   Lemma qc : SelectionConforms wf_schema q wf_schema.(query_type).
   Proof.
@@ -276,12 +273,7 @@ Section Example.
          by [].
   Qed.  *)
 
-  Lemma qwf : is_query_wf q.
-  Proof. by []. Qed.
-
-  Let wf_query := WFQuery qwf.
-  
-  Lemma qbc : wf_query_conforms wf_schema wf_query wf_schema.(query_type).
+  Lemma qbc : selection_conforms wf_schema q wf_schema.(query_type).
   Proof. by []. Qed.
 
 
@@ -291,94 +283,102 @@ Section Example.
 
 
 
-  Let query_response := (NestedResult "hero"
-                                       (ResponseList
-                                          [::
-                                             (SingleResult "name" "Luke");
-                                             (NestedListResult "friends"
-                                               [::
-                                                  (ResponseList
-                                                     [::
-                                                        Empty;
-                                                        ResponseList
-                                                          [::
-                                                             (SingleResult "droidFriend" "R2-D2");
-                                                             (SingleResult "primaryFunction" "Astromech")
-                                                          ]
-                                                     ]
-                                                  );
-                                                  (ResponseList
-                                                     [::
-                                                        (ResponseList
-                                                           [::
-                                                              (SingleResult "humanFriend" "Han");
-                                                              (NestedListResult "starships"
-                                                                                [::
-                                                                                   (ResponseList
-                                                                                      [::
-                                                                                         (SingleResult "starship" "Falcon");
-                                                                                         (SingleResult "length" "34.37")
-                                                                                      ]
-                                                                                   )
-                                                                                ]
-                                                              )
-                                                           ]
-                                                        );
-                                                        Empty
-                                                     ]  
-                                                     
-                                                  )
-                                               ]
-                                             )
-                                          ]
-                         )).
+  Let query_response :=
+    (SingleResponse
+       (NestedResult "hero"
+          (MultipleResponses
+             (SingleResult "name" "Luke")
+             (SingleResponse
+                (NestedListResult "friends"
+                   [::
+                      (MultipleResponses
+                         (SingleResult "droidFriend" "R2-D2")
+                         (MultipleResponses
+                            (SingleResult "primaryFunction" "Astromech")
+                            (SingleResponse Empty)
+                          )
+                      );
+                      (MultipleResponses
+                         Empty
+                         (MultipleResponses
+                            (SingleResult "humanFriend" "Han")
+                            (SingleResponse
+                               (NestedListResult "starships"
+                                  [::
+                                     (MultipleResponses
+                                        (SingleResult "starship" "Falcon")
+                                        (SingleResponse (SingleResult "length" "34.37"))
+                                     )
+                                  ]
+                               )
+                            )
+                         )  
+                      )
+                   ]
+                )
+             )
+          )
+       )
+    ).
      
 
 
    
 
                 
-    Example ev_query_eq_response :  (eval_query  wf_graph conformed_query) = query_response.
+    Example ev_query_eq_response :  (eval_selection  wf_graph conformed_query) = query_response.
     Proof.
-      rewrite /eval_query /=.
+      rewrite /eval_selection /eval /=.
       rewrite /get_target_nodes_with_field /=.
       rewrite /edges [fset]unlock /=.
-      do ?[rewrite ?collect_equation ?/indexed_map /=].
-      by []. 
-    Qed.
+      do ?[rewrite ?collect_eq ?/indexed_map /=]. by [].
+      Admitted.
+    
 
 
-    Let q' := (NestedField "hero" [fmap ("episode", "EMPIRE")]
-                          (SelectionSet
-                             [::
-                                (SingleField "name" emptym);
-                                
-                                (SingleField "name" emptym);
-                                     
-                                (SingleField "id" emptym);
-                                (SingleField "name" emptym)
-                             ]
-                          )
-                          
-             ).
+    Let q' :=
+      (SingleSelection
+         (NestedField "hero" [fmap ("episode", "EMPIRE")]
+            (MultipleSelection
+               (SingleField "name" emptym)
+               (MultipleSelection
+                  (SingleField "name" emptym)
+                  (MultipleSelection                  
+                     (SingleField "id" emptym)
+                     (SingleSelection (SingleField "name" emptym))
+                  )
+               )
+            )
+         )
+      ).
 
-    Lemma qwf' : is_query_wf q'.
-        by []. Qed.
-    Let wf_query' := WFQuery qwf'.
-             
-     Lemma qbc' : wf_query_conforms wf_schema wf_query' wf_schema.(query_type).
+     Lemma qbc' : selection_conforms wf_schema q' wf_schema.(query_type).
   Proof. by []. Qed.
   
 
 
     Let conformed_query' := ConformedQuery qbc'. 
 
-    Goal (eval_query wf_graph conformed_query') = (NestedResult "hero" (ResponseList [:: (SingleResult "name" "Luke"); (SingleResult "id" "1000")])).
-      rewrite /eval_query /=.
+    Goal (eval_selection wf_graph conformed_query') =
+    (SingleResponse
+       (NestedResult "hero"
+                     (MultipleResponses
+                        (SingleResult "name" "Luke")
+                        (MultipleResponses
+                           Empty
+                           (MultipleResponses
+                              (SingleResult "id" "1000")
+                              (SingleResponse Empty)
+                           )
+                        )
+                     )
+       )
+    ).
+      rewrite /eval_selection /eval /=.
       rewrite /get_target_nodes_with_field /=.
       rewrite /edges [fset]unlock /=.
-      by do ?[rewrite ?collect_equation ?/indexed_map /=]. 
-    Qed.
+      do ?[rewrite ?collect_eq ?/indexed_map /=].  by [].
+      Admitted.
 
     Example ex7 :
       let r := [::
